kore/src/Freshness.v
@@ -5,8 +5,9 @@ Section Freshness.
   Context {Σ : Signature}.
 
   Fixpoint free_evars {ex mu s}
+                      (sTarget : sort)
                       (φ : Pattern ex mu s)
-                      (sTarget : sort) {struct φ} : gset (evar sTarget) :=
+                      {struct φ} : gset (evar sTarget) :=
   match φ with
    | @kore_fevar _ _ _ var_sort x =>
        (* var_sort = s in this case *)
@@ -17,20 +18,21 @@ Section Freshness.
    | kore_imp φ1 φ2 | kore_iff φ1 φ2
    | kore_and φ1 φ2 | kore_or φ1 φ2
    | kore_equals _ φ1 φ2 | kore_in _ φ1 φ2
-      => free_evars φ1 sTarget ∪ free_evars φ2 sTarget
+      => free_evars sTarget φ1 ∪ free_evars sTarget φ2
    | kore_app σ args
-      => hlist_rect ∅ (fun _ _ x xs rest => free_evars x sTarget ∪ rest) args
+      => hlist_rect ∅ (fun _ _ x xs rest => free_evars sTarget x ∪ rest) args
    | kore_exists _ φ | kore_forall _ φ
    | kore_mu φ | kore_nu φ 
    | kore_not φ | kore_ceil _ φ | kore_floor _ φ
-      => free_evars φ sTarget
+      => free_evars sTarget φ
    | kore_bevar _ | kore_fsvar _ | kore_bsvar _
    | kore_bot _ | kore_top _ => ∅
   end.
 
   Fixpoint free_svars {ex mu s}
+                      (sTarget : sort)
                       (φ : Pattern ex mu s)
-                      (sTarget : sort) {struct φ} : gset (svar sTarget) :=
+                      {struct φ} : gset (svar sTarget) :=
   match φ with
    | @kore_fsvar _ _ _ var_sort X =>
        (* var_sort = s in this case *)
@@ -41,13 +43,13 @@ Section Freshness.
    | kore_imp φ1 φ2 | kore_iff φ1 φ2
    | kore_and φ1 φ2 | kore_or φ1 φ2
    | kore_equals _ φ1 φ2 | kore_in _ φ1 φ2
-      => free_svars φ1 sTarget ∪ free_svars φ2 sTarget
+      => free_svars sTarget φ1 ∪ free_svars sTarget φ2
    | kore_app σ args
-      => hlist_rect ∅ (fun _ _ x xs rest => free_svars x sTarget ∪ rest) args
+      => hlist_rect ∅ (fun _ _ x xs rest => free_svars sTarget x ∪ rest) args
    | kore_exists _ φ | kore_forall _ φ
    | kore_mu φ | kore_nu φ 
    | kore_not φ | kore_ceil _ φ | kore_floor _ φ
-      => free_svars φ sTarget
+      => free_svars sTarget φ
    | kore_bevar _ | kore_fevar _ | kore_bsvar _
    | kore_bot _ | kore_top _ => ∅
   end.
@@ -55,10 +57,26 @@ Section Freshness.
   Definition fresh_evar {s} {ex mu}
       (sTarget : sort) (φ : Pattern s ex mu) :
       evar sTarget :=
-    fresh (elements (free_evars φ sTarget)).
+    fresh (elements (free_evars sTarget φ)).
   Definition fresh_svar {s} {ex mu}
       (sTarget : sort) (φ : Pattern s ex mu) :
       svar sTarget :=
-    fresh (elements (free_svars φ sTarget)).
+    fresh (elements (free_svars sTarget φ)).
+
+  Lemma fresh_evar_is_fresh {s} {ex mu} (sTarget : sort) (φ : Pattern s ex mu) :
+    fresh_evar sTarget φ ∉ free_evars sTarget φ.
+  Proof.
+    unfold fresh_evar.
+    pose proof (is_fresh (free_evars sTarget φ)).
+    set_solver.
+  Defined.
+
+  Lemma fresh_svar_is_fresh {s} {ex mu} (sTarget : sort) (φ : Pattern s ex mu) :
+    fresh_svar sTarget φ ∉ free_svars sTarget φ.
+  Proof.
+    unfold fresh_evar.
+    pose proof (is_fresh (free_svars sTarget φ)).
+    set_solver.
+  Defined.
 
 End Freshness.
